Another example for siobhan

michael_formal/Syntax.thy
@@ -14,6 +14,18 @@ definition Leq :: "aexp \<Rightarrow> aexp \<Rightarrow> bexp" (infix "\<le>" 60
   "Leq a b = (Not (Gt a b))"
 declare Leq_def [simp]
 
+definition and_infix :: "bexp \<Rightarrow> bexp \<Rightarrow> bexp" (infix "\<and>" 60) where
+  "and_infix a b = And a b"
+declare and_infix_def [simp]
+
+definition eq_infix :: "aexp \<Rightarrow> aexp \<Rightarrow> bexp" (infix "=" 100) where
+  "eq_infix a b = And (Not (Gt a b)) (Not (Gt b a))"
+declare eq_infix_def [simp]
+
+definition plus :: "aexp \<Rightarrow> aexp \<Rightarrow> aexp" (infix "+" 65) where
+  "plus a b = Plus a b"
+declare plus_def [simp]
+
 definition true :: guard  where
   "true = [(Bc True)]"
 declare true_def [simp]
