michael_formal/Lift.thy
@@ -1,0 +1,101 @@
+theory Lift
+  imports EFSM
+begin
+definition t1up :: "transition" where
+"t1up \<equiv> \<lparr>
+        Label = ''goUp'',
+        Arity = 1,
+        Guard = [((V ''i1'') > (N 0))],
+        Outputs = [(''o1'', V ''i1'')],
+        Updates = []
+      \<rparr>"
+
+definition t2up :: "transition" where
+"t2up \<equiv> \<lparr>
+        Label = ''goUp'',
+        Arity = 1,
+        Guard = [((V ''i1'') > (N 0))],
+        Outputs = [(''o1'', ((V ''i1'') + (N (-1))))],
+        Updates = []
+      \<rparr>"
+
+definition t3up :: "transition" where
+"t3up \<equiv> \<lparr>
+        Label = ''goUp'',
+        Arity = 1,
+        Guard = [((V ''r1'') = (N 0))],
+        Outputs = [(''o1'', N 0)],
+        Updates = []
+      \<rparr>"
+
+definition t1down :: "transition" where
+"t1down \<equiv> \<lparr>
+        Label = ''goDown'',
+        Arity = 1,
+        Guard = [((V ''i1'') > (N 0))],
+        Outputs = [(''o1'', V ''i1'')],
+        Updates = []
+      \<rparr>"
+
+definition t2down :: "transition" where
+"t2down \<equiv> \<lparr>
+        Label = ''goDown'',
+        Arity = 1,
+        Guard = [((V ''i1'') > (N 0))],
+        Outputs = [(''o1'', ((V ''i1'') + (N (-1))))],
+        Updates = []
+      \<rparr>"
+
+definition t3down :: "transition" where
+"t3down \<equiv> \<lparr>
+        Label = ''goDown'',
+        Arity = 1,
+        Guard = [((V ''r1'') = (N 0))],
+        Outputs = [(''o1'', N 0)],
+        Updates = []
+      \<rparr>"
+
+definition openDoors :: transition where
+"openDoors \<equiv> \<lparr>
+        Label = ''open'',
+        Arity = 0,
+        Guard = true,
+        Outputs = [(''o1'', N 1)],
+        Updates = []
+      \<rparr>"
+
+definition closeDoors :: transition where
+"closeDoors \<equiv> \<lparr>
+        Label = ''close'',
+        Arity = 0,
+        Guard = true,
+        Outputs = [(''o1'', N 0)],
+        Updates = []
+      \<rparr>"
+
+lemmas transitions = t1up_def t2up_def t3up_def t1down_def t2down_def t3down_def openDoors_def closeDoors_def
+
+definition lift :: "efsm" where
+"lift \<equiv> \<lparr> S = [1,2,3,4],
+          s0 = 1,
+          T = \<lambda> (a,b) . 
+                   if (a,b) = (1,2) then [t1up]
+              else if (a,b) = (2,2) then [t2up]
+              else if (a,b) = (2,1) then [t3up]
+              else if (a,b) = (1,3) then [t1down]
+              else if (a,b) = (3,3) then [t2down]
+              else if (a,b) = (3,1) then [t3down]
+              else if (a,b) = (1,4) then [openDoors]
+              else if (a,b) = (4,1) then [closeDoors]
+              else []
+         \<rparr>"
+
+lemma "observe_trace lift (s0 lift) <> [(''goUp'', [1]), (''goUp'', [0]), (''open'', [])] = [[1], [0], [1]]"
+  by (simp add: step_def lift_def transitions join_def index_def shows_stuff input2state_def)
+
+lemma "observe_trace lift (s0 lift) <> [(''goDown'', [1]), (''goDown'', [0]), (''open'', [])] = [[1], [0], [1]]"
+  by (simp add: step_def lift_def transitions join_def index_def shows_stuff input2state_def)
+
+lemma "observe_trace lift (s0 lift) <> [(''open'', []), (''close'', []), (''open'', [])] = [[1], [0], [1]]"
+  by (simp add: step_def lift_def transitions join_def index_def shows_stuff input2state_def)
+end
